refinedVST/typing/adequacy.v
@@ -196,3 +196,50 @@ Ltac adequacy_solve_typed_function lemma unfold_tac :=
     adequacy_intro_parameter => /=; repeat (constructor; [done|]); by constructor |
     | iApply lemma => //; iExists _; repeat iSplit => //];
     adequacy_intro_parameter => /=; eexists eq_refl => /=; split_and!; [..|adequacy_intro_parameter => /=; split_and!];  repeat adequacy_solve_equiv unfold_tac.*)
+
+(* export to base triples *)
+Definition fn_params_pre `{!VSTGS OK_ty Σ} {cs : compspecs} {A} fn fp (x : @dtfr Σ A) lsa : assert :=
+  ⎡([∗ list] v;'(cty, t) ∈ lsa;zip (map snd (fn_params fn)) (fp_atys (fp x)), v ◁ᵥₐₗ| cty | t) ∗ fp_Pa (fp x)⎤.
+
+Definition fn_params_post `{!VSTGS OK_ty Σ} {cs : compspecs} {A} fn fp (x : @dtfr Σ A) v : assert :=
+  ∃ ty, (⎡opt_ty_own_val (fn_return fn) ty v⎤ -∗ ∃ y, ⎡opt_ty_own_val (fn_return fn) ((fp x).(fp_fr) y).(fr_rty) v⎤ ∗ ⎡((fp x).(fp_fr) y).(fr_R)⎤).
+
+Lemma typed_function_triple : forall `{!VSTGS OK_ty Σ} {cs : compspecs} {A} Espec ge f fp
+    (Hcomplete : Forall (λ it, composite_compute.complete_legal_cosu_type it.2 = true) (fn_vars f))
+    (Halign : Forall (λ it, align_mem.LegalAlignasFacts.LegalAlignasDefs.is_aligned cenv_cs ha_env_cs la_env_cs it.2 0 = true) (fn_vars f))
+    (Hvolatile : Forall (λ it, type_is_volatile it.2 = false) (fn_vars f)),
+  ⎡typed_function Espec ge f fp⎤ ⊢ ∀ x : dtfr A, fun_triple Espec (Build_genv ge cenv_cs) (fn_params_pre f fp x) f (fn_params_post f fp x).
+Proof.
+  rewrite /fun_triple /fn_params_pre /=; intros.
+  iIntros "#?" (?) "!> %% ? H0 ?"; rewrite (stackframe_of_typed(typeG0 := VST_typeG)) //.
+  iApply wp_strong_mono.
+  iSplitL "H0". 2: {
+    iStopProof; split => n; monPred.unseal; rewrite monPred_at_intuitionistically.
+    iIntros "(H & (Hargs & ?) & Hstack)".
+    iDestruct ("H" $! x) as "(%Htys & #H)".
+    pose proof (tc_vals_length _ _ H) as Hlen; rewrite map_length in Hlen.
+    apply Forall2_length in Htys as ->; rewrite Hlen.
+    iApply ("H" $! _ (Vector.of_list args)).
+    rewrite vec_to_list_to_vec; iFrame. }
+  rewrite /= /Clight_seplog.bind_ret; iSplit.
+  - rewrite /fn_params_post /=.
+    iIntros "($ & H) !>"; iFrame.
+    iDestruct ("H" with "[//]") as "(% & $ & ? & $)".
+    iExists tytrue; iIntros "_"; iFrame.
+  - do 2 (iSplit; first by iIntros "[]").
+    rewrite /fn_params_post /=.
+    iIntros (?) "(% & Hret & % & H)".
+    iDestruct ("H" with "Hret") as "(% & ? & ? & $)"; iFrame.
+    (* typed ret is inconsistent with function_body_ret_assert *)
+Admitted.
+
+Lemma typed_fptr_triple : forall `{!VSTGS OK_ty Σ} {cs : compspecs} {A} Espec ge fp l cty,
+  ⎡l ◁ᵥₐₗ|cty| function_ptr Espec ge fp⎤ ⊢ ∃ f, ⌜Genv.find_funct ge l = Some (Internal f)⌝ ∧ ∀ x : dtfr A, ▷ fun_triple Espec (Build_genv ge cenv_cs) (fn_params_pre f fp x) f (fn_params_post f fp x).
+Proof.
+  rewrite /ty_own_val_at /ty_own_val /= /ty_own_val /=.
+  intros.
+  iIntros "(%x & % & (-> & %) & %Hfn & H)"; simpl in *; subst.
+  destruct x, Hfn as (? & ? & ? & ? & ? & ? & ? & ? & ?); subst; simpl.
+  iExists _; iSplit; first by iPureIntro; apply Genv.find_funct_ptr_iff.
+  rewrite -bi.later_forall embed_later; by iPoseProof (typed_function_triple with "H") as "H".
+Qed.
